Progress with the Hybrid Machine Proof.

concurrency/HybridMachine_simulation_proof.v
@@ -1,11 +1,13 @@
-From mathcomp.ssreflect Require Import ssreflect seq ssrbool ssrfun.
 Require Import compcert.common.AST.
 Require Import Coq.omega.Omega.
 Require Import Clight.
 Require Import Memory.
 Require Import Values.
 Require Import Globalenvs.
-Require Import Compiler.
+
+Require Import Coq.Classes.Morphisms.
+
+Require Import compcert.driver.Compiler.
 Require Import compcert.lib.Coqlib.
 
 Require Import msl.Coqlib2.
@@ -14,6 +16,8 @@ Require veric.Clight_core. Import Clight_core.
 
 Require Import Smallstep.
 Require Import ExposedSmallstep.
+Require Import concurrency.SantiagosTactics.
+Require Import concurrency.MemoryEquivalences.
 Require Import concurrency.x86_context.
 Require Import concurrency.concurrent_machine.
 Require Import concurrency.HybridMachine.
@@ -88,6 +92,55 @@ Section OneThreadCompiled.
       self_simulation (Asm_semantics tp) _ (Asm.State).  
     Definition code_inject_target:=
       match_self (code_inject Asm_self_simulation).
+    
+
+    Instance mem_Proper_match_perm_image:
+      Proper (eq ==> mem_equiv ==> mem_equiv ==> iff) perm_image.
+    Proof.
+      proper_iff_tac; intros; subst.
+      intros ??; rewrite <- H0; eapply H2.
+    Qed.
+    Instance mem_Proper_match_perm_preimage:
+      Proper (eq ==> mem_equiv ==> mem_equiv ==> iff) perm_preimage.
+    Proof.
+      proper_iff_tac; intros; subst.
+      intros ???; rewrite <- H1 in *.
+      destruct (H2 _ _ H) as (b1 & delta & ofs & ?).
+      do 3 eexists.
+      rewrite <- H0; eauto.
+    Qed.
+
+    Instance mem_Proper_match_mem:
+        Proper (eq ==> mem_equiv ==> mem_equiv ==> iff) match_mem.
+      Proof.
+        proper_iff_tac; intros; subst.
+        inversion H2.
+        econstructor; eauto;
+          rewrite <- H0, <- H1; auto.
+      Qed.
+    
+    Instance mem_Proper_code_inject_target:
+      Proper (eq ==> eq ==> mem_equiv ==> eq ==> mem_equiv ==> iff) code_inject_target.
+    Proof.
+      proper_iff_tac; intros; subst.
+      econstructor; try rewrite <- H1, <- H3;
+        ez_eapply code_inject_target.
+    Qed.
+
+    
+    Instance mem_Proper_code_inject_source:
+      Proper (eq ==> eq ==> mem_equiv ==> eq ==> mem_equiv ==> iff) code_inject_source.
+    Proof.
+      proper_iff_tac; intros; subst.
+      econstructor; try rewrite <- H1, <- H3;
+        ez_eapply code_inject_source.
+    Qed.
+                      
+                        
+                  
+                  
+          
+    
     
     (* Definition code_inject_source:=
       self_simulation.code_inject _ _ (Clight_self_simulation p). *)
@@ -262,6 +315,20 @@ Section OneThreadCompiledMatch.
       match_thread_compiled cd j (Kinit v1 v1') m1
                             (Kinit v2 v2') m2.
 
+  Definition FST {A B} (HH : A /\ B):=
+    fst (ssrfun.pair_of_and HH).
+
+  Definition SND {A B} (HH : A /\ B):=
+    snd (ssrfun.pair_of_and HH).
+  
+(*
+  Definition FST {A B} (HH : A /\ B) : A:=
+    match HH with
+    | conj H _ => H
+    end. *)
+
+  
+
   Record concur_match (ocd: option compiler_index)
        (j:meminj) (cstate1: C1) (m1: mem) (cstate2: C2) (m2: mem):=
   { same_length: num_threads cstate1 = num_threads cstate2
@@ -270,31 +337,34 @@ Section OneThreadCompiledMatch.
     ; mtch_source:
         forall (i:nat),
           (i > hb')%nat ->
-          forall (cnti1: containsThread cstate1 i),
+          forall (cnti1: containsThread cstate1 i)
+            (cnti2: containsThread cstate2 i),
           match_thread_source  j
                               (getThreadC cnti1)
-                              (restrPermMap (memcompat1 i cnti1).1)
-                              (getThreadC (same_length_contains same_length cnti1))
-                              (restrPermMap (memcompat2 i (same_length_contains same_length cnti1)).1)
+                              (restrPermMap (FST (memcompat1 i cnti1)))
+                              (getThreadC cnti2)
+                              (restrPermMap (FST (memcompat2 i cnti2)))
     ; mtch_target:
         forall (i:nat),
           (i < hb')%nat ->
-          forall (cnti1: containsThread cstate1 i),
+          forall (cnti1: containsThread cstate1 i)
+            (cnti2: containsThread cstate2 i),
           match_thread_target  j
                               (getThreadC cnti1)
-                              (restrPermMap (memcompat1 i cnti1).1)
-                              (getThreadC (same_length_contains same_length cnti1))
-                              (restrPermMap (memcompat2 i (same_length_contains same_length cnti1)).1)
+                              (restrPermMap (FST(memcompat1 i cnti1)))
+                              (getThreadC cnti2)
+                              (restrPermMap (FST(memcompat2 i cnti2)))
     ; mtch_compiled:
         forall (i:nat),
           (i = hb')%nat ->
-          forall (cnti1: containsThread cstate1 i),
+          forall (cnti1: containsThread cstate1 i)
+            (cnti2: containsThread cstate2 i),
             exists cd, ocd = Some cd /\
           match_thread_compiled cd j
                                 (getThreadC cnti1)
-                                (restrPermMap (memcompat1 i cnti1).1)
-                                (getThreadC (same_length_contains same_length cnti1))
-                                (restrPermMap (memcompat2 i (same_length_contains same_length cnti1)).1) }.
+                                (restrPermMap (FST(memcompat1 i cnti1)))
+                                (getThreadC cnti2)
+                                (restrPermMap (FST(memcompat2 i cnti2))) }.
 
 Lemma contains12:
   forall {data j cstate1 m1 cstate2 m2},
@@ -328,7 +398,346 @@ Arguments memcompat2 {ocd j cstate1 m1 cstate2 m2}.
     Notation the_simulation := compiler_simulation.
 
     Parameter option_compiler_order: option (Injindex the_simulation) -> option (Injindex the_simulation) -> Prop.
+
+    (* automatic rewrite gsoThreadCode *)
+    Ltac auto_gsoThreadCode:=
+      match goal with
+      | [ |- context[getThreadC ?cntJ'] ] =>
+        match type of cntJ' with
+        | containsThread (updThread ?cntI _ _) ?J =>
+          match type of cntI with
+          | containsThread ?hb ?I =>
+            match goal with
+            | [ cntJ: containsThread hb J |- _ ] => 
+              rewrite gsoThreadCode with
+                  (cnti:= cntI)
+                  (cntj:= cntJ)
+                  (cntj':= cntJ') by eassumption
+            end
+          end
+        end  
+      end.
+    Ltac simpl_getThreadC':=
+      first[ rewrite gssThreadCode |
+             auto_gsoThreadCode
+           ].
+
+    (*Produces all the "containThreads" that might be missing "*)
+    Ltac containsThread_helper:=
+      match goal with
+      | [ cntj': containsThread (updThread ?cntj _ _) ?i  |- _ ] =>
+        match type of cntj with
+        | containsThread ?hb ?j =>
+          progress (
+              first [match goal with
+                     | [ cnti: containsThread hb i |- _ ] => idtac
+                     end |
+                     let CNTI:= fresh "cnti" in
+                     assert (CNTI: containsThread hb i)
+                       by
+                         (eapply cntUpdate'; eapply cntj') ])
+        | _ => fail
+        end 
+      end.
     
+    Ltac simpl_getThreadC:=
+      match goal with
+      | [  |- context [@getThreadC _ _ ?j (@updThread _ _ _ ?hb _ _ _) _ ] ] =>
+        let cntJ:= fresh "cntj" in
+        evar (cntj : containsThread hb j);
+        let cntJ':= eval unfold cntJ in cntJ in
+            rewrite gsoThreadCode with
+            (tp := hb)
+            (cntj:= cntJ')
+          by eassumption;
+                                        instantiate (cntJ:= ltac:(eauto));
+                                        clear cntJ
+      end.
+    
+    Ltac containsThread_cleanup:=
+      repeat match goal with
+             | [H1: containsThread ?TP ?M,
+                    H2: containsThread (@updThread _ _ _ ?TP _ _ _) ?M |- _] =>
+               replace H2 with H1 in * by apply proof_irr; clear H2
+             | [H1: containsThread ?TP ?M,
+                    H2: containsThread ?TP ?M |- _] =>
+               replace H2 with H1 in * by apply proof_irr; clear H2
+             end.
+
+    Lemma mem_step_same_visible:
+                  forall hb Sems Semt i j tp1 tp2 m1 m2
+                    (cnti1: containsThread tp1 i)
+                    (cntj1: containsThread tp1 j)
+                    (cnti2: containsThread tp2 i)
+                  (compat1: HybridMachine.mem_compatible hb Sems Semt tp1 m1)
+                  (compat2: HybridMachine.mem_compatible hb Sems Semt tp2 m2),
+                    j <> i ->
+                    semantics.mem_step (restrPermMap (FST (compat1 j cntj1))) m2 ->
+                  same_visible (restrPermMap (FST (compat1 i cnti1)))
+                               (restrPermMap (FST (compat2 i cnti2))).
+                Proof.
+                  (*SKETCH:
+                   * mem_step ensures only writable memory is modified.
+                   * mem_compatible (compat1) ensures that the writable memory 
+                   * for thread j is disjoint from the visible memory for thread i
+                   * Concluding that visible memory for i is unmodified.  
+                   *)
+                Admitted.
+                
+                Lemma match_thread_source_same_vis:
+                  forall f f' m1 m1' m2 m2' cs ct,
+                  same_visible m1 m1' ->
+                  same_visible m2 m2' ->
+                   is_ext f (Mem.nextblock m1) f' (Mem.nextblock m2) ->
+                  match_thread_source f cs m1 ct m2 ->
+                  match_thread_source f' cs m1' ct m2'.
+                Proof.
+                  (*SKETCH:
+                   * There are some holes with regards to at_ext and after_ext
+                   * Otherwise, source_match is invariant under changes to non_visible memory.
+                   *)
+                Admitted.
+                Lemma match_thread_compiled_same_vis:
+                  forall f f' m1 m1' m2 m2' cs ct cd,
+                  same_visible m1 m1' ->
+                  same_visible m2 m2' ->
+                  is_ext f (Mem.nextblock m1) f' (Mem.nextblock m2) ->
+                  match_thread_compiled cd f cs m1 ct m2 ->
+                  match_thread_compiled cd f' cs m1' ct m2'.
+                Proof.
+                  (*SKETCH:
+                   * There are some holes with regards to at_ext and after_ext
+                   * Otherwise, source_match is invariant under changes to non_visible memory.
+                   *)
+                Admitted.
+                Lemma match_thread_target_same_vis:
+                  forall f f' m1 m1' m2 m2' cs ct,
+                  same_visible m1 m1' ->
+                  same_visible m2 m2' ->
+                   is_ext f (Mem.nextblock m1) f' (Mem.nextblock m2) ->
+                  match_thread_target f cs m1 ct m2 ->
+                  match_thread_target f' cs m1' ct m2'.
+                Proof.
+                  (*SKETCH:
+                   * There are some holes with regards to at_ext and after_ext
+                   * Otherwise, source_match is invariant under changes to non_visible memory.
+                   *)
+                Admitted.
+
+                
+            Lemma mem_step_compatible:
+                forall hb1 Sems Semt c m m' code_i i
+                  (cnti: containsThread c i) 
+                  (Hcmpt1: HybridMachine.mem_compatible hb1 Sems Semt c m),
+                  semantics.mem_step (restrPermMap (FST (Hcmpt1 i cnti))) m'->
+                  HybridMachine.mem_compatible hb1 Sems Semt
+                                               (updThread cnti
+                                                          code_i
+                                                          (getCurPerm m', (snd (getThreadR cnti)))) m'.
+            Admitted.
+            Lemma gss_restrPermMap:
+              forall Sems Semt hb i (tp: t_ (ThreadPool hb Sems Semt)) m c
+                (cnti: containsThread tp i)
+                (COMPT: HybridMachine.mem_compatible hb Sems Semt
+                        (updThread cnti c (getCurPerm m, snd (getThreadR cnti))) m),
+                mem_equiv (restrPermMap (FST (COMPT i cnti))) m.
+            Proof.
+              intros; constructor.
+              - intros.
+                pose proof (restrPermMap_contents (FST (COMPT i cnti))).
+                unfold juicy_mem.contents_at in H.
+                match type of H with
+                  ?LHS = ?RHS =>
+                  let lhs:= fresh lhs in
+                  remember LHS as lhs;
+                    let rhs:= fresh rhs in
+                    remember RHS as rhs;
+                      assert (forall b ofs,
+                                 (lhs) (b, ofs) = (rhs) (b,ofs))
+                      by (intros; rewrite H; reflexivity);
+                      subst lhs rhs
+                end.
+                apply H0.
+              - intros.
+                destruct kind.
+                + pose proof (restrPermMap_Max (FST (COMPT i cnti))) as HH.
+                  unfold permission_at in HH; rewrite HH; auto.
+                  rewrite getMaxPerm_correct; reflexivity.
+                + pose proof (restrPermMap_Cur (FST (COMPT i cnti))) as HH.
+                  unfold permission_at in HH; rewrite HH.
+                  cbv delta[getThreadR_ ThreadPool OrdinalThreadPool_rec] zeta iota beta.
+                  simpl.
+                  match goal with
+                  | [ |- context[if ?DEC then _ else _] ] =>
+                    destruct DEC eqn:DECC
+                  end.
+                  * simpl; rewrite getCurPerm_correct; reflexivity.
+                  * clear -DECC; exfalso.
+                    unfold eqtype.eq_op,eqtype.Equality.op in DECC; simpl in DECC.
+                    rewrite <- ssrnat.eqnE in DECC.
+                    pose proof (@ssrnat.eqnP i i) as HH.
+                    rewrite DECC in HH.
+                    inversion HH.
+                    apply H; auto.
+              - reflexivity.
+            Qed.
+            Lemma concur_stable_thread_step_target:
+              forall  cd f (c1:C1) m1 c2 m2 f' ts1' m1' ts2' m2' tid,
+              forall (Htid1: containsThread c1 tid)
+                (Htid2: containsThread c2 tid)
+                (LT : (tid < hb')%nat)
+                (Hcmpt1: HybridMachine.mem_compatible hb1 Sems Semt c1 m1)
+                (Hcmpt2: HybridMachine.mem_compatible hb2 Sems Semt c2 m2),
+                concur_match cd f c1 m1 c2 m2 ->
+                is_ext f (Mem.nextblock m1) f' (Mem.nextblock m2) ->
+                semantics.mem_step (restrPermMap (FST (Hcmpt1 _ Htid1))) m1' ->
+                semantics.mem_step (restrPermMap (FST (Hcmpt2 _ Htid2))) m2' ->
+                match_self (code_inject Asm_self_simulation) f' ts1' m1' ts2' m2' ->
+                concur_match cd f'
+                             (updThread Htid1  (Krun (TState _ _ ts1')) (getCurPerm m1', (snd (getThreadR Htid1))))  m1'
+                             (updThread Htid2 (Krun (TState _ _ ts2')) (getCurPerm m2', (snd (getThreadR Htid2)))) m2'.
+            Proof.
+              (*Oct 9: Sketching the proof... *)
+              intros.
+              (*First set up some results *)
+              remember (updThread Htid1 (Krun (TState (semC Sems) Asm.regset ts1'))
+                                  (getCurPerm m1', (snd (getThreadR Htid1)))) as cstates1'.
+              remember (updThread Htid2 (Krun (TState (semC Sems) Asm.regset ts2'))
+                                  (getCurPerm m2', (snd(getThreadR Htid2)))) as cstates2'.
+              assert (SAME: num_threads cstates1' = num_threads cstates2') by (subst; apply H).
+              assert (COMPAT1: HybridMachine.mem_compatible hb1 Sems Semt cstates1' m1').
+              subst cstates1'.
+              (*mem_step preserves coherence *)
+              
+              eapply mem_step_compatible; eauto.
+              assert (COMPAT2:HybridMachine.mem_compatible hb2 Sems Semt cstates2' m2').
+              subst cstates2'.
+              eapply mem_step_compatible; eauto.
+              eapply (Build_concur_match _ _ _ _ _ _ SAME COMPAT1 COMPAT2).
+              (*In each of the following cases, one should look at {i = tid} + {i <> tid}*)
+              - (* (i > hb') *)
+                intros.
+                assert (tid <> i) by omega.
+                
+                subst.
+                repeat containsThread_helper.
+                assert (cnti1 = cnti0) by apply proof_irr.
+                subst cnti1.
+                assert (cnti2 = cnti) by apply proof_irr.
+                subst cnti2.
+                do 2 simpl_getThreadC.
+                
+                eapply match_thread_source_same_vis.
+
+                {
+                eapply mem_step_same_visible.
+                + eassumption.
+                + eapply H1.
+                }
+                {  
+                eapply mem_step_same_visible.
+                + eassumption.
+                + eapply H2.
+                }
+                eauto.
+                
+                assert (Hcmpt1 = memcompat1 H) by apply proof_irr; subst Hcmpt1.
+                assert (Hcmpt2 = memcompat2 H) by apply proof_irr; subst Hcmpt2.
+                eapply H; auto.
+                
+                
+              - (* (i < hb') *)
+                intros.
+                destruct (NPeano.Nat.eq_dec i tid).
+                
+                + (* i = tid *)
+                  subst tid.
+                  subst cstates1' cstates2'.
+                  do 2 rewrite gssThreadCode.
+                  econstructor.
+                  clear - H3.
+                  fold code_inject_target in H3.
+                  
+                  dup COMPAT1.
+                  containsThread_cleanup.
+                  do 2 rewrite gss_restrPermMap; auto.
+
+                  
+                + (* i <> tid *)
+                  assert (tid <> i) by omega.
+
+                  subst.
+                  repeat containsThread_helper.
+                  assert (cnti1 = cnti0) by apply proof_irr.
+                  subst cnti1.
+                  assert (cnti2 = cnti) by apply proof_irr.
+                  subst cnti2.
+                  do 2 simpl_getThreadC.
+                  
+                  eapply match_thread_target_same_vis.
+                  
+
+                  
+                {
+                eapply mem_step_same_visible.
+                + eassumption.
+                + eapply H1.
+                }
+                {  
+                eapply mem_step_same_visible.
+                + eassumption.
+                + eapply H2.
+                }
+                eauto.
+                
+                assert (Hcmpt1 = memcompat1 H) by apply proof_irr; subst Hcmpt1.
+                assert (Hcmpt2 = memcompat2 H) by apply proof_irr; subst Hcmpt2.
+                eapply H; auto.
+                  
+              - (* (i = hb') *)
+                intros.
+                assert (tid <> i) by omega.
+
+                subst.
+                repeat containsThread_helper.
+                assert (cnti1 = cnti) by apply proof_irr.
+                subst cnti1.
+                assert (cnti2 = cnti0) by apply proof_irr.
+                subst cnti2.
+                do 2 simpl_getThreadC.
+
+                exploit (mtch_compiled _ _ _ _ _ _ H).
+                reflexivity.
+                intros [cd' [? ?]].
+                exists (cd'); split; eauto.
+                
+                eapply match_thread_compiled_same_vis.
+                {
+                eapply mem_step_same_visible.
+                + eassumption.
+                + eapply H1.
+                }
+                {  
+                eapply mem_step_same_visible.
+                + eassumption.
+                + eapply H2.
+                }
+                eauto.
+
+                assert (Hcmpt1 = memcompat1 H) by apply proof_irr; subst Hcmpt1.
+                assert (Hcmpt2 = memcompat2 H) by apply proof_irr; subst Hcmpt2.
+
+                eapply H6.
+            Qed.
+            Lemma Asm_mem_semantics:
+              forall genv c1 m1 t c2 m2
+                (Astep: Asm.step genv (Asm.State c1 m1) t (Asm.State c2 m2)),
+                semantics.mem_step m1 m2.
+            Proof. intros. 
+            Admitted.
+            
+            
+                
     Lemma hybrid_thread_diagram:
       forall (U0 : list nat) (st1 : C1) (m1 : mem) (st1' : C1) (m1' : mem),
         machine_semantics.thread_step (HCSem Sems Semt hb1 U) genv U0 st1 m1 st1' m1' ->
@@ -351,23 +760,34 @@ Arguments memcompat2 {ocd j cstate1 m1 cstate2 m2}.
         destruct (Compare_dec.lt_eq_lt_dec (tid) hb') as [[LT | EQ] | LT ].
         
         + (* tid < hb' *)
-          (*This case it's all in target*)
+          (*This case it's all in target (the step is in target?) *)
+          assert (LT':=LT).
           inversion Htstep. subst tp' m' ev0.
           eapply event_semantics.ev_step_ax1 in Hcorestep.
           assert (MSTEP:= semantics.corestep_mem _ _ _ _ _ _ Hcorestep). 
           simpl in Hcorestep.
           simpl in Hcode.
-          eapply H0 in LT. instantiate (1 := Htid) in LT.
+          assert (cnti2: containsThread st2 tid).
+          eapply same_length_contains; simpl in Htid; eauto; eapply H0.
+          
+          eapply H0 in LT.  
+          
+          instantiate (1:=cnti2) in LT.
+          instantiate (1:=Htid) in LT.
+          
+
           rewrite Hcode in LT.
           assert (Htid':= contains12 H0 Htid).
           inv LT. 
           
-          
+
+          rename H5 into SSIM.
           (*Use the source self_simulations*)
           inversion Hcorestep; subst.
-          eapply (ssim_diagram) in H5; eauto; simpl in H5.
+          eapply (ssim_diagram) in SSIM; eauto; simpl in SSIM.
           Focus 2.
           {
+            (*SHOW the step*)
             replace (memcompat1 H0) with Hcmpt by (apply proof_irr); simpl; eauto.
             clear - H4.
             
@@ -375,10 +795,10 @@ Arguments memcompat2 {ocd j cstate1 m1 cstate2 m2}.
             inversion H4;
               try solve[eapply Asm.exec_step_internal; eauto];
               try solve[eapply Asm.exec_step_builtin; eauto].
-          } Unfocus.
+          } Unfocus. 
           
-          simpl in H5.
-          destruct H5 as [c2' [f' [t' [m2' [STEP [SMATCH [EXT TINJ]]]]]]].
+          simpl in SSIM.
+          destruct SSIM as [c2' [f' [t' [m2' [STEP [SMATCH [EXT TINJ]]]]]]].
          
 
         exists (@updThread_ _ _ _ _ st2 Htid'
@@ -392,36 +812,28 @@ Arguments memcompat2 {ocd j cstate1 m1 cstate2 m2}.
         
         split.
           * (*Reestablish the match*)
-            Lemma concur_stable_thread_step_target:
-              forall  cd f (c1:C1) m1 c2 m2 f' c1' m1' c2' m2' tid,
-              forall (Htid1: containsThread c1 tid)
-                (Htid2: containsThread c2 tid)
-                (Hcmpt1: HybridMachine.mem_compatible hb1 Sems Semt c1 m1)
-                (Hcmpt2: HybridMachine.mem_compatible hb2 Sems Semt c2 m2),
-                concur_match cd f c1 m1 c2 m2 ->
-                is_ext f (Mem.nextblock m1) f' (Mem.nextblock m2) ->
-                semantics.mem_step (restrPermMap (Hcmpt1 _ Htid1)#1) m1' ->
-                semantics.mem_step (restrPermMap (Hcmpt2 _ Htid2)#1) m2' ->
-                match_self (code_inject Asm_self_simulation) f' c1' m1' c2' m2' ->
-                concur_match cd f'
-                             (updThread Htid1  (Krun (TState _ _ c1')) (getCurPerm m1', (getThreadR Htid1)#2))  m1'
-                             (updThread Htid2 (Krun (TState _ _ c2')) (getCurPerm m2', (getThreadR Htid2)#2)) m2'.
-            Admitted.
             eapply concur_stable_thread_step_target; eauto.
-            -- admit. (*Follows from mem_sem and the step proven in the follwoing goal*)
-            
+            containsThread_cleanup.
+            eapply Asm_mem_semantics; eauto.
+
           (*Prove the machine step*)
           * left.
             eapply machine_semantics_lemmas.thread_step_plus_one.
             econstructor; simpl; eauto.
             econstructor; eauto.
-        -- admit. (*Invariant: going to need to add this to the match relation *)
-        -- inversion TINJ; subst.
-           econstructor; simpl. 
-           instantiate (3 := (memcompat2 H0)).
-           (*Have the step STEP, but have to show it's an internal step!*)
-           admit.
-        -- simpl; repeat f_equal. apply proof_irr. apply proof_irr.
+            -- admit. (*Invariant: going to need to add this to the match relation *)
+            -- inversion TINJ; subst.
+               econstructor; simpl. 
+               instantiate (3 := (memcompat2 H0)).
+               simpl in SMATCH.
+               (*Have the step STEP, but have to show it's an internal step!*)
+               (*This can be a lemma or an axiom of self-simulation*)
+               admit.
+               (*NOTE: acctually, look at ssim_diagram, used to get SSIM.*)
+            (*And look at the SHOW the step proof above.  *)
+               (* The simulation semantics should have the propery of mantaining*)
+               (* internall-external steps *)
+            -- simpl; repeat f_equal. apply proof_irr. apply proof_irr.
 
         
         + (* tid = hb' *)
@@ -432,7 +844,7 @@ Arguments memcompat2 {ocd j cstate1 m1 cstate2 m2}.
           simpl in Hcorestep.
           assert (Hcode':= Hcode).
           simpl in Hcode.
-          eapply H0 in EQ. instantiate (1 := Htid) in EQ.
+          eapply H0 in EQ. 
           rewrite Hcode in EQ.
           assert (Htid':= contains12 H0 Htid).
           destruct EQ as [cd0 [cd_eq EQ]]; inv EQ.
@@ -440,6 +852,38 @@ Arguments memcompat2 {ocd j cstate1 m1 cstate2 m2}.
                           f1 & f2 & f3 &
                           INJsrc & INJcomp & INJtgt &
                           compose).
+          
+          
+          Lemma compiled_thread_diagram:
+            forall (U0 : list nat) (st1 : C1) (m1 m1' : mem) (tid : nat)
+                   (Htid : containsThread_ (ThreadPool hb1 Sems Semt) st1 tid) (c' : semC (Sem hb1 Sems Semt))
+                   (st2 : C2) (mu : meminj) (m2 : mem) (cd0 : compiler_index)
+                   (H0 : concur_match (Some cd0) mu st1 m1 st2 m2) (code1 : CC_core) 
+                   (code2 : Asm.regset) (st1_ : CC_core) (m1_ : mem)
+                   (st2_ : X86Machines.ErasedMachine.ThreadPool.code) (m2_ : mem) 
+                   (f1 f2 f3 : meminj) cnti2,
+              source_match f1 code1 (restrPermMap (FST ((memcompat1 H0) tid Htid))) st1_ m1_ ->
+              compiler_match cd0 f2 (make_state_Clight st1_ m1_) (make_state_Asm st2_ m2_) ->
+              target_match f3 code2
+                           (restrPermMap
+                              (FST
+                                 ((memcompat2 H0) tid
+                                                  cnti2))) st2_
+                           m2_ ->
+              exists (st2' : C2) (m2' : mem) (cd' : option compiler_index) (mu' : meminj),
+                concur_match cd' mu'
+                             (updThread_ (ThreadPool hb1 Sems Semt) Htid (Krun c')
+                                         (getCurPerm m1', snd (getThreadR_ (ThreadPool hb1 Sems Semt) Htid))) m1' st2' m2' /\
+                (machine_semantics_lemmas.thread_step_plus (HCSem Sems Semt hb2 U) genv 
+                                                           (tid :: U0) st2 m2 st2' m2' \/
+                 machine_semantics_lemmas.thread_step_star (HCSem Sems Semt hb2 U) genv 
+                                                           (tid :: U0) st2 m2 st2' m2' /\ option_compiler_order cd' (Some cd0)).
+          Proof.
+            intros.
+            
+          
+          
+          (*LOOK HERE!!! *)
           (*Have to apply a self simulation, then the compiler simulation
             and then a self simulation again. *)
           admit. (*TODO: Make this a Lemma compiled_thread_diagram*)
@@ -519,17 +963,18 @@ Arguments memcompat2 {ocd j cstate1 m1 cstate2 m2}.
   End HybridThreadDiagram.
 
   Section MachineThreadDiagram.
-    
+
+    (*One threas takes a "machine step" (or synchronization-step) *)
     Lemma machine_thread_diagram:
       forall (U0 : seq.seq nat) (tr : seq.seq machine_event) (st1 : C1) 
     (m1 : mem) (U' : seq.seq nat) (tr' : seq.seq machine_event) (st1' : C1) 
     (m1' : mem),
-  machine_semantics.machine_step (HCSem Sems Semt hb1 U) genv U0 tr st1 m1 U' tr' st1' m1' ->
-  forall (cd : option (Injindex compiler_simulation)) (st2 : C2) (mu : meminj) (m2 : mem),
-  concur_match cd mu st1 m1 st2 m2 ->
-  exists (st2' : C2) (m2' : mem) (cd' : option (Injindex compiler_simulation)),
-    concur_match cd' mu st1' m1' st2' m2' /\
-    machine_semantics.machine_step (HCSem Sems Semt hb2 U) genv U0 tr st2 m2 U' tr' st2' m2'.
+        machine_semantics.machine_step (HCSem Sems Semt hb1 U) genv U0 tr st1 m1 U' tr' st1' m1' ->
+        forall (cd : option (Injindex compiler_simulation)) (st2 : C2) (mu : meminj) (m2 : mem),
+          concur_match cd mu st1 m1 st2 m2 ->
+          exists (st2' : C2) (m2' : mem) (cd' : option (Injindex compiler_simulation)),
+            concur_match cd' mu st1' m1' st2' m2' /\
+            machine_semantics.machine_step (HCSem Sems Semt hb2 U) genv U0 tr st2 m2 U' tr' st2' m2'.
     Proof.
       intros.
       destruct U0 as [|i U0]; simpl in H.
@@ -714,10 +1159,9 @@ Arguments memcompat2 {ocd j cstate1 m1 cstate2 m2}.
               _ option_compiler_order
               (concur_match)  v.
   Proof.
-    
   exists Vundef.
   econstructor.
-  - admit. (*eapply Injfsim_order_wf*)
+  - admit. (*eapply Injfsim_order_wf *)
   - (* core_initial*)
     admit.
     (*
@@ -740,8 +1184,7 @@ Arguments memcompat2 {ocd j cstate1 m1 cstate2 m2}.
     intros.
     eapply hybrid_thread_diagram; eauto.
   - (*machine_diagram*)
-    (* eapply machine_thread_diagram; eauto. *)
-    admit.
+     eapply machine_thread_diagram; eauto.
   - (*thread_halted *)
     admit.
     
